MutualExclusion.v
@@ -9,30 +9,30 @@ From Elo Require Import Waiting.
 From Elo Require Import Holding.
 
 (* ------------------------------------------------------------------------- *)
-(* unique-holding                                                            *)
+(* mutual-exclusion                                                          *)
 (* ------------------------------------------------------------------------- *)
 
-Definition unique_holding (m : mem) (ths : threads) := forall ad,
+Definition mutual_exclusion (m : mem) (ths : threads) := forall ad,
   (m[ad].X = false -> forall_threads ths (not_holding ad)) /\
   (m[ad].X = true  -> forone_thread  ths (holding ad) (not_holding ad)).
 
 (* lemmas ------------------------------------------------------------------ *)
 
-Corollary hg_or_nhg_from_uhg : forall ad m ths tid,
-  unique_holding m ths ->
+Corollary hg_or_nhg_from_mu : forall ad m ths tid,
+  mutual_exclusion m ths ->
   holding ad ths[tid] \/ not_holding ad ths[tid].
 Proof.
-  intros * Huhg. specialize (Huhg ad) as [? Htrue].
+  intros * Hmu. specialize (Hmu ad) as [? Htrue].
   destruct (m[ad].X); spec; eauto.
   specialize Htrue as [tid' [? ?]].
   nat_eq_dec tid' tid; auto.
 Qed.
 
-Corollary nocr_or_onecr_from_uhg : forall ad m ths tid,
-  unique_holding m ths ->
+Corollary nocr_or_onecr_from_mu : forall ad m ths tid,
+  mutual_exclusion m ths ->
   no_cr ad ths[tid] \/ one_cr ad ths[tid].
 Proof.
-  intros * Huhg. specialize (Huhg ad) as [Hfalse Htrue].
+  intros * Hmu. specialize (Hmu ad) as [Hfalse Htrue].
   destruct (m[ad].X); spec.
   - specialize Htrue as [tid' [[? ?] Hnhg]].
     nat_eq_dec tid' tid; auto.
@@ -40,15 +40,15 @@ Proof.
   - specialize (Hfalse tid). destruct Hfalse as [? | [? ?]]; eauto.
 Qed.
 
-Corollary uhg_hg_contradiction : forall ad m ths tid1 tid2,
-  unique_holding m ths ->
+Corollary mu_hg_contradiction : forall ad m ths tid1 tid2,
+  mutual_exclusion m ths ->
   (* --- *)
   tid1 <> tid2 ->
   holding ad ths[tid1] ->
   holding ad ths[tid2] ->
   False.
 Proof.
-  intros * Huhg **. specialize (Huhg ad) as [? Htrue].
+  intros * Hmu **. specialize (Hmu ad) as [? Htrue].
   destruct (m[ad].X); spec;
   eauto using hg_contradiction.
   specialize Htrue as [tid [? ?]].
@@ -56,39 +56,39 @@ Proof.
   eauto using hg_contradiction.
 Qed.
 
-Corollary uhg_hg_equality : forall ad m ths tid1 tid2,
-  unique_holding m ths ->
+Corollary mu_hg_equality : forall ad m ths tid1 tid2,
+  mutual_exclusion m ths ->
   (* --- *)
   holding ad ths[tid1] ->
   holding ad ths[tid2] ->
   tid1 = tid2.
 Proof.
   intros. nat_eq_dec tid1 tid2; trivial. exfalso.
-  eauto using uhg_hg_contradiction.
+  eauto using mu_hg_contradiction.
 Qed.
 
 Lemma locked_from_holding : forall m ths tid ad,
-  unique_holding m ths ->
+  mutual_exclusion m ths ->
   (* --- *)
   holding ad ths[tid] ->
   m[ad].X = true.
 Proof.
-  intros * Huhg ?.
+  intros * Hmu ?.
   destruct (m[ad].X) eqn:Heq; trivial.
-  specialize (Huhg ad) as [? _]. spec.
+  specialize (Hmu ad) as [? _]. spec.
   exfalso. eauto using hg_contradiction.
 Qed.
 
 Lemma locked_from_rel : forall m ths tid t ad,
   forall_threads ths (valid_term m) ->
-  unique_holding m ths     ->
+  mutual_exclusion m ths     ->
   (* --- *)
   ths[tid] --[e_rel ad]--> t ->
   m[ad].X = true.
 Proof.
-  intros * ? Huhg ?.
+  intros * ? Hmu ?.
   destruct (m[ad].X) eqn:Heq; trivial.
-  specialize (Huhg ad) as [Hnholding _]. spec.
+  specialize (Hmu ad) as [Hnholding _]. spec.
   exfalso. specialize (Hnholding tid) as [? | [? ?]];
   eauto using nocr_rel_contradiction, wg_effect_contradiction.
 Qed.
@@ -96,55 +96,44 @@ Qed.
 Lemma locked_from_wrel : forall m ths tid t ad,
   forall_threads ths (valid_term m) ->
   forall_threads ths (consistent_waits WR_none) ->
-  unique_holding m ths     ->
+  mutual_exclusion m ths     ->
   (* --- *)
   ths[tid] --[e_wrel ad]--> t ->
   m[ad].X = true.
 Proof.
-  intros * ? ? Huhg ?.
+  intros * ? ? Hmu ?.
   destruct (m[ad].X) eqn:Heq; trivial.
-  specialize (Huhg ad) as [Hnholding _]. spec.
+  specialize (Hmu ad) as [Hnholding _]. spec.
   exfalso. specialize (Hnholding tid) as [? | [? ?]];
   eauto using nocr_wrel_contradiction, wg_effect_contradiction.
 Qed.
 
-(* preservation lemmas ----------------------------------------------------- *)
-
-Lemma uhg_mem_region : forall m ths ad R,
-  unique_holding m ths ->
-  unique_holding m[ad.R <- R] ths.
-Proof.
-  intros * H. intros ad'. specialize (H ad').
-  repeat omicron; upsilon; destruct H; trivial;
-  split; repeat intro; repeat omicron; upsilon; spec; eauto.
-Qed.
-
 (* preservation ------------------------------------------------------------ *)
 
-Local Lemma uhg_preservation_none : forall m ths tid t,
+Local Lemma mu_preservation_none : forall m ths tid t,
   forall_threads ths (valid_term m) ->
   (* --- *)
   tid < #ths ->
-  unique_holding m ths ->
+  mutual_exclusion m ths ->
   ths[tid] --[e_none]--> t ->
-  unique_holding m ths[tid <- t].
+  mutual_exclusion m ths[tid <- t].
 Proof.
   intros until 1.
-  intros ? Huhg ? ad. specialize (Huhg ad) as [Hfall Hfone].
+  intros ? Hmu ? ad. specialize (Hmu ad) as [Hfall Hfone].
   split; intros; spec.
   - intros ?. omicron; eauto using nhg_preservation_none.
   - specialize Hfone as [tid' [? ?]]. exists tid'. split; intros; omicron;
     eauto using nhg_preservation_none, hg_preservation_none.
 Qed.
 
-Local Lemma uhg_preservation_alloc : forall m ths tid t T R,
+Local Lemma mu_preservation_alloc : forall m ths tid t T R,
   tid < #ths ->
-  unique_holding m ths ->
+  mutual_exclusion m ths ->
   ths[tid] --[e_alloc (#m) T]--> t ->
-  unique_holding (m +++ new_cell T R) ths[tid <- t].
+  mutual_exclusion (m +++ new_cell T R) ths[tid <- t].
 Proof.
   intros *.
-  intros ? Huhg ? ad. specialize (Huhg ad) as [Hfall Hfone].
+  intros ? Hmu ? ad. specialize (Hmu ad) as [Hfall Hfone].
   split; intros; upsilon; spec.
   - intros ?. omicron; eauto using nhg_preservation_alloc.
   - specialize Hfone as [tid' [? ?]]. exists tid'.
@@ -152,16 +141,16 @@ Proof.
     eauto using nhg_preservation_alloc, hg_preservation_alloc.
 Qed.
 
-Local Lemma uhg_preservation_init : forall m ths tid t ad' t',
+Local Lemma mu_preservation_init : forall m ths tid t ad' t',
   forall_threads ths (valid_term m) ->
   (* --- *)
   tid < #ths ->
-  unique_holding m ths ->
+  mutual_exclusion m ths ->
   ths[tid] --[e_init ad' t']--> t ->
-  unique_holding m[ad'.t <- t'] ths[tid <- t].
+  mutual_exclusion m[ad'.t <- t'] ths[tid <- t].
 Proof.
   intros until 1.
-  intros ? Huhg ? ad. specialize (Huhg ad) as [Hfall Hfone].
+  intros ? Hmu ? ad. specialize (Hmu ad) as [Hfall Hfone].
   assert (ad' < #m) by eauto using vtm_init_address.
   split; intros; omicron; upsilon; spec; solve
     [ intro; omicron; eauto using nhg_preservation_init
@@ -171,17 +160,17 @@ Proof.
     ].
 Qed.
 
-Local Lemma uhg_preservation_read : forall m ths tid t ad te,
+Local Lemma mu_preservation_read : forall m ths tid t ad te,
   value te ->
   valid_term m te ->
   (* --- *)
   tid < #ths ->
-  unique_holding m ths ->
+  mutual_exclusion m ths ->
   ths[tid] --[e_read ad te]--> t ->
-  unique_holding m ths[tid <- t].
+  mutual_exclusion m ths[tid <- t].
 Proof.
   intros until 2.
-  intros ? Huhg ? ad'. specialize (Huhg ad') as [Hfall Hfone].
+  intros ? Hmu ? ad'. specialize (Hmu ad') as [Hfall Hfone].
   split; intros; upsilon; spec.
   - intros ?. omicron; eauto using nhg_preservation_read.
   - specialize Hfone as [tid' [? ?]]. exists tid'.
@@ -189,16 +178,16 @@ Proof.
     eauto using nhg_preservation_read, hg_preservation_read.
 Qed.
 
-Local Lemma uhg_preservation_write : forall m ths tid t ad te,
+Local Lemma mu_preservation_write : forall m ths tid t ad te,
   forall_threads ths (valid_term m) ->
   (* --- *)
   tid < #ths ->
-  unique_holding m ths ->
+  mutual_exclusion m ths ->
   ths[tid] --[e_write ad te]--> t ->
-  unique_holding m[ad.t <- te] ths[tid <- t].
+  mutual_exclusion m[ad.t <- te] ths[tid <- t].
 Proof.
   intros until 1.
-  intros ? Huhg ? ad'. specialize (Huhg ad') as [Hfall Hfone].
+  intros ? Hmu ? ad'. specialize (Hmu ad') as [Hfall Hfone].
   assert (ad < #m) by eauto using vtm_write_address.
   split; intros; repeat omicron; spec; upsilon;
   eauto using nhg_unit, nhg_preservation_write;
@@ -206,7 +195,7 @@ Proof.
   omicron; eauto using nhg_preservation_write, hg_preservation_write.
 Qed.
 
-Local Lemma uhg_preservation_acq : forall m ths tid ad t te,
+Local Lemma mu_preservation_acq : forall m ths tid ad t te,
   value te ->
   valid_term m te ->
   forall_threads ths (valid_term m) ->
@@ -214,12 +203,12 @@ Local Lemma uhg_preservation_acq : forall m ths tid ad t te,
   (* --- *)
   m[ad].X = false ->
   tid < #ths ->
-  unique_holding m ths ->
+  mutual_exclusion m ths ->
   ths[tid] --[e_acq ad te]--> t ->
-  unique_holding m[ad.X <- true] ths[tid <- t].
+  mutual_exclusion m[ad.X <- true] ths[tid <- t].
 Proof.
   intros until 5.
-  intros ? Huhg ? ad'. specialize (Huhg ad') as [Hfall Hfone].
+  intros ? Hmu ? ad'. specialize (Hmu ad') as [Hfall Hfone].
   assert (ad < #m) by eauto using vtm_acq_address.
   split; intros; repeat omicron; spec; upsilon;
   eauto using nhg_unit, nhg_preservation_acq.
@@ -238,16 +227,16 @@ Proof.
     + intros. omicron; eauto using nhg_preservation_acq.
 Qed.
 
-Local Lemma uhg_preservation_rel : forall m ths tid ad t,
+Local Lemma mu_preservation_rel : forall m ths tid ad t,
   forall_threads ths (valid_term m) ->
   (* --- *)
   tid < #ths ->
-  unique_holding m ths ->
+  mutual_exclusion m ths ->
   ths[tid] --[e_rel ad]--> t ->
-  unique_holding m[ad.X <- false] ths[tid <- t].
+  mutual_exclusion m[ad.X <- false] ths[tid <- t].
 Proof.
   intros until 1.
-  intros ? Huhg ? ad'. destruct (Huhg ad') as [Hfall Hfone].
+  intros ? Hmu ? ad'. destruct (Hmu ad') as [Hfall Hfone].
   assert (Had : m[ad].X = true) by eauto using locked_from_rel.
   split; intros; try intros tid'; repeat omicron; spec; upsilon;
   auto; eauto using nhg_preservation_rel;
@@ -265,18 +254,18 @@ Proof.
     + omicron; eauto using nhg_preservation_rel.
 Qed.
 
-Local Lemma uhg_preservation_wacq : forall m ths tid t ad,
+Local Lemma mu_preservation_wacq : forall m ths tid t ad,
   forall_threads ths (valid_term m) ->
   forall_threads ths (consistent_waits WR_none) ->
   (* --- *)
   m[ad].X = false ->
   tid < #ths ->
-  unique_holding m ths ->
+  mutual_exclusion m ths ->
   ths[tid] --[e_wacq ad]--> t ->
-  unique_holding m[ad.X <- true] ths[tid <- t].
+  mutual_exclusion m[ad.X <- true] ths[tid <- t].
 Proof.
   intros until 3.
-  intros ? Huhg ? ad'. specialize (Huhg ad') as [Hfall Hfone].
+  intros ? Hmu ? ad'. specialize (Hmu ad') as [Hfall Hfone].
   assert (ad < #m) by eauto using vtm_wacq_address.
   split; intros; repeat omicron; spec; upsilon;
   eauto using nhg_unit, nhg_preservation_wacq.
@@ -288,24 +277,24 @@ Proof.
       * specialize (Hfall tid) as [? | [? ?]].
         ** eauto using nocr_preservation_wacq, cw_preservation_wacq,
             noreacq_from_nocr1.
-        ** eauto using wg_to_noreacq.
+        ** eauto using noreacq_from_wacq.
     + intros. sigma. eauto.
   - specialize Hfone as [tid' [? ?]]. exists tid'. split.
     + omicron; eauto using hg_preservation_wacq.
     + intros. omicron; eauto using nhg_preservation_wacq.
 Qed.
 
-Local Lemma uhg_preservation_wrel : forall m ths tid ad t,
+Local Lemma mu_preservation_wrel : forall m ths tid ad t,
   forall_threads ths (valid_term m) ->
   forall_threads ths (consistent_waits WR_none) ->
   (* --- *)
   tid < #ths ->
-  unique_holding m ths ->
+  mutual_exclusion m ths ->
   ths[tid] --[e_wrel ad]--> t ->
-  unique_holding m[ad.X <- false] ths[tid <- t].
+  mutual_exclusion m[ad.X <- false] ths[tid <- t].
 Proof.
   intros until 2.
-  intros ? Huhg ? ad'. destruct (Huhg ad') as [Hfall Hfone].
+  intros ? Hmu ? ad'. destruct (Hmu ad') as [Hfall Hfone].
   assert (Had : m[ad].X = true) by eauto using locked_from_wrel.
   split; intros; try intros tid'; repeat omicron; spec; upsilon;
   auto; eauto using nhg_preservation_wrel;
@@ -327,16 +316,16 @@ Qed.
 Local Ltac eapply_in_tstep tt :=
   match goal with Htstep : _ --[_]--> _ |- _ => eapply tt in Htstep as ? end.
 
-Local Lemma uhg_preservation_spawn : forall m ths tid t t',
+Local Lemma mu_preservation_spawn : forall m ths tid t t',
   forall_threads ths (valid_term m) ->
   (* --- *)
   tid < #ths ->
-  unique_holding m ths ->
+  mutual_exclusion m ths ->
   ths[tid] --[e_spawn t']--> t ->
-  unique_holding m (ths[tid <- t] +++ t').
+  mutual_exclusion m (ths[tid <- t] +++ t').
 Proof.
   intros until 1.
-  intros ? Huhg ? ad'. destruct (Huhg ad') as [Hfall Hfone].
+  intros ? Hmu ? ad'. destruct (Hmu ad') as [Hfall Hfone].
   split; intros; spec.
   - intro. omicron;
     eauto using nhg_preservation_spawn, nhg_unit.
@@ -349,32 +338,32 @@ Proof.
       left. eauto using nocr_spawn_term.
 Qed.
 
-Theorem uhg_preservation_cstep : forall m1 m2 ths1 ths2 tid e,
+Theorem mu_preservation_cstep : forall m1 m2 ths1 ths2 tid e,
   forall_memory  m1 value                ->
   forall_program m1 ths1 (valid_term m1) ->
   forall_program m1 ths1 (consistent_waits WR_none) ->
   (* --- *)
-  unique_holding m1 ths1 ->
+  mutual_exclusion m1 ths1 ->
   m1 \ ths1 ~~[tid, e]~~> m2 \ ths2 ->
-  unique_holding m2 ths2.
+  mutual_exclusion m2 ths2.
 Proof.
   intros * ? [? ?] [? ?] **. invc_cstep; try invc_mstep.
-  - eauto using uhg_preservation_none.
-  - sigma. upsilon. eauto using uhg_preservation_alloc.
-  - eauto using uhg_preservation_init.
-  - eauto using uhg_preservation_read.
-  - eauto using uhg_preservation_write.
-  - eauto using uhg_preservation_acq.
-  - eauto using uhg_preservation_rel.
-  - eauto using uhg_preservation_wacq.
-  - eauto using uhg_preservation_wrel.
-  - eauto using uhg_preservation_spawn.
+  - eauto using mu_preservation_none.
+  - sigma. upsilon. eauto using mu_preservation_alloc.
+  - eauto using mu_preservation_init.
+  - eauto using mu_preservation_read.
+  - eauto using mu_preservation_write.
+  - eauto using mu_preservation_acq.
+  - eauto using mu_preservation_rel.
+  - eauto using mu_preservation_wacq.
+  - eauto using mu_preservation_wrel.
+  - eauto using mu_preservation_spawn.
 Qed.
 
-Theorem uhg_preservation_base : forall t,
+Theorem mu_preservation_base : forall t,
   no_crs t ->
   (* --- *)
-  unique_holding nil (base t).
+  mutual_exclusion nil (base t).
 Proof.
   unfold base. intros ** ?. split; intros Hnil.
   - intro. left. omicron; auto using no_cr.
