InheritanceNoReacq.v
@@ -1,0 +1,84 @@
+From Elo Require Import Core.
+
+From Elo Require Import NoReacq.
+From Elo Require Import ValidTerm.
+
+(* ------------------------------------------------------------------------- *)
+
+Local Ltac solve_noreacq_inheritance :=
+  intros; ind_tstep; repeat invc_vtm; repeat invc_noreacq;
+  eauto using noreacq_from_value, no_reacq.
+
+Lemma noreacq_inheritance_none : forall ad m t1 t2,
+  valid_term m t1 ->
+  (* --- *)
+  no_reacq ad t2 ->
+  t1 --[e_none]--> t2 ->
+  no_reacq ad t1.
+Proof. solve_noreacq_inheritance. Qed.
+
+Lemma noreacq_inheritance_alloc : forall ad t1 t2 ad' T',
+  no_reacq ad t2 ->
+  t1 --[e_alloc ad' T']--> t2 ->
+  no_reacq ad t1.
+Proof. solve_noreacq_inheritance. Qed.
+
+Lemma noreacq_inheritance_init : forall ad m t1 t2 ad' t',
+  valid_term m t1 ->
+  (* --- *)
+  no_reacq ad t2 ->
+  t1 --[e_init ad' t']--> t2 ->
+  no_reacq ad t1.
+Proof. solve_noreacq_inheritance. Qed.
+
+Lemma noreacq_inheritance_read : forall ad t1 t2 ad' t',
+  no_reacq ad t' ->
+  (* --- *)
+  no_reacq ad t2 ->
+  t1 --[e_read ad' t']--> t2 ->
+  no_reacq ad t1.
+Proof. solve_noreacq_inheritance. Qed.
+
+Lemma noreacq_inheritance_write : forall ad m t1 t2 ad' t',
+  valid_term m t1 ->
+  (* --- *)
+  no_reacq ad t2 ->
+  t1 --[e_write ad' t']--> t2 ->
+  no_reacq ad t1.
+Proof. solve_noreacq_inheritance. Qed.
+
+Lemma noreacq_inheritance_acq : forall ad m t1 t2 ad' t',
+  valid_term m t1 ->
+  (* --- *)
+  no_reacq ad t2 ->
+  t1 --[e_acq ad' t']--> t2 ->
+  no_reacq ad t1.
+Proof. solve_noreacq_inheritance. Qed.
+
+Lemma noreacq_inheritance_rel : forall ad t1 t2 ad',
+  no_reacq ad t2 ->
+  t1 --[e_rel ad']--> t2 ->
+  no_reacq ad t1.
+Proof. solve_noreacq_inheritance. Qed.
+
+Lemma noreacq_inheritance_wacq : forall ad t1 t2 ad',
+  ad <> ad' ->
+  no_reacq ad t2 ->
+  t1 --[e_wacq ad']--> t2 ->
+  no_reacq ad t1.
+Proof. solve_noreacq_inheritance. Qed.
+
+Lemma noreacq_inheritance_wrel : forall ad t1 t2 ad',
+  no_reacq ad t2 ->
+  t1 --[e_wrel ad']--> t2 ->
+  no_reacq ad t1.
+Proof. solve_noreacq_inheritance. Qed.
+
+Lemma noreacq_inheritance_spawn : forall ad m t1 t2 t',
+  valid_term m t1 ->
+  (* --- *)
+  no_reacq ad t2 ->
+  t1 --[e_spawn t']--> t2 ->
+  no_reacq ad t1.
+Proof. solve_noreacq_inheritance. Qed.
+
