Safety.v
@@ -11,6 +11,8 @@ From Elo Require Import GCR.
 From Elo Require Import HappensBefore.
 From Elo Require Import SafetyLemmas.
 
+Notation "'<<' ev1 ',' tc ',' ev2 '>>'" := (ev2 :: tc +++ ev1).
+
 Local Lemma in_app_head : forall {A} (l : list A) (a : A),
   In a (l ++ a :: nil).
 Proof.
@@ -130,24 +132,6 @@ Ltac destruct_ustep3 :=
 (* TODO                                                                      *)
 (* ------------------------------------------------------------------------- *)
 
-(* TODO: posso usar consistent_term *)
-Local Lemma uninitialized_from_oneinit : forall m ths tid ad,
-  forall_threads ths (valid_term m) ->
-  unique_initializers m ths ->
-  (* --- *)
-  one_init ad ths[tid] ->
-  m[ad].t = None.
-Proof.
-  intros * ? Hui ?.
-  assert (Had : ad < #m) by eauto using oneinit_ad_bound.
-  destruct (Hui ad Had). opt_dec (m[ad].t); trivial.
-  spec. exfalso. eauto using noinit_oneinit_contradiction.
-Qed.
-
-(* ------------------------------------------------------------------------- *)
-(* TODO                                                                      *)
-(* ------------------------------------------------------------------------- *)
-
 Local Lemma destruct_ustep' : forall m1 m2 ths1 ths2 tc1 tc2 tid e,
   m1 \ ths1 ~~[tc2 ++ (tid, e) :: tc1]~~>* m2 \ ths2 ->
   exists mA mB thsA thsB,
@@ -198,24 +182,25 @@ Qed.
 (* one-init ~~>* one-cr                                                      *)
 (* ------------------------------------------------------------------------- *)
 
-(*
+(* TODO *)
 Local Lemma oneinit_multistep_onecr_requires_acq' :
   forall m1 m2 ths1 ths2 tid1 tid2 tc ad,
     invariants m1 ths1 ->
     invariants m2 ths2 ->
     (* --- *)
-    tid1 <> tid2 ->
-    one_init ad ths1[tid1] ->
+    tid1 <> tid2                   ->
+    one_init ad ths1[tid1]         ->
     m1 \ ths1 ~~[tc]~~>* m2 \ ths2 ->
-    one_cr ad ths2[tid2] ->
+    holding ad ths2[tid2]          ->
     exists t, In (tid2, (e_acq ad t)) tc.
 Proof.
-  intros. ind_ustep.
-  - exfalso.
+  intros * ? ? ? ? ? Hhg. ind_ustep.
+  - exfalso. destruct Hhg.
     assert (Hice : init_cr_exclusivity ths) by eauto with inva.
     specialize (Hice ad tid1 tid2) as [? _].
     eauto using nocr_onecr_contradiction.
-  - assert (invariants m2 ths2) by eauto using invariants_preservation_ustep.
+  - (* TODO: now that we have holding, we can revisit safety lemma. *)
+    assert (invariants m2 ths2) by eauto using invariants_preservation_ustep.
     repeat spec.
     assert (exists t, (e <> e_acq ad t /\ one_cr ad ths2[tid2]) \/
                       (e =  e_acq ad t /\ tid = tid2))
@@ -257,10 +242,10 @@ Proof.
   intros * ? ? ? H.
   eapply destruct_ustep' in H. decompose record H.
   repeat eexists; eauto.
-  invc_cstep. invc_cstep. invc_mstep. eauto.
+  invc_rstep. invc_cstep. invc_mstep. eauto.
 Qed.
 
-Local Lemma oneinit_multistep_initialized_requires_init :
+Local Lemma oneinit_multistep_initialized_requires_insert :
   forall tc m1 m2 ths1 ths2 tid ad t,
     invariants m1 ths1 ->
     invariants m2 ths2 ->
@@ -268,7 +253,7 @@ Local Lemma oneinit_multistep_initialized_requires_init :
     one_init ad ths1[tid] ->
     m1 \ ths1 ~~[tc]~~>* m2 \ ths2 ->
     m2[ad].t = Some t ->
-    exists t, In (tid, e_init ad t) tc.
+    exists t, In (tid, e_insert ad t) tc.
 Proof.
   intro. induction tc using rev_ind; intros.
   - invc_ustep.
@@ -282,13 +267,13 @@ Proof.
       eapply destruct_ustep' in H as [mA [mB [thsA [thsB [H1A [? ?]]]]]]
     end.
     invc H1A.
-    assert (invariants mB thsB) by eauto using invariants_preservation_cstep.
+    assert (invariants mB thsB) by eauto using invariants_preservation_rstep.
     specialize (IHtc mB m2 thsB ths2 tid ad t). do 2 spec.
     assert (
-      (forall t, e' <> e_init ad t /\ one_init ad thsB[tid]) \/
-      (exists t, e' =  e_init ad t /\ tid' = tid /\ mB[ad].t = Some t)
+      (forall t, e' <> e_insert ad t /\ one_init ad thsB[tid]) \/
+      (exists t, e' =  e_insert ad t /\ tid' = tid /\ mB[ad].t = Some t)
     ) as [H' | [t' [? [? _]]]]
-      by eauto using oneinit_preservation_cstep.
+      by eauto using oneinit_preservation_rstep.
       + specialize (H' t) as [? Honeinit].
         specialize IHtc as [t' Hin]; trivial.
         eauto using in_app_tail.
@@ -306,7 +291,7 @@ Local Lemma oneinit_multistep_onecr :
     one_cr   ad ths2[tid2]         ->
     exists tc1 tc2 t t',
       tc = tc2 ++ tc1               /\
-      In (tid1, e_init ad t') tc1 /\
+      In (tid1, e_insert ad t') tc1 /\
       In (tid2, e_acq    ad t)  tc2.
 Proof.
   intros.
@@ -319,15 +304,14 @@ Proof.
     as [mA [thsA [? [? ?]]]]
     by eauto using multistep_acq_requires_initialized.
   assert (invariants mA thsA) by eauto using invariants_preservation_ustep.
-  assert (exists t, In (tid1, e_init ad t) tc1)
+  assert (exists t, In (tid1, e_insert ad t) tc1)
     as [t' ?]
-    by eauto using oneinit_multistep_initialized_requires_init.
+    by eauto using oneinit_multistep_initialized_requires_insert.
   exists tc1. exists (tc2 ++ (tid2, e_acq ad t) :: nil).
   exists t. exists t'.
   repeat split; eauto using in_app_head.
   rewrite <- app_assoc. reflexivity.
 Qed.
-*)
 
 (* ------------------------------------------------------------------------- *)
 (* one-cr ~~>* one-init                                                      *)
@@ -367,318 +351,51 @@ Proof.
 Qed.
 
 (* ------------------------------------------------------------------------- *)
-(* one-cr ~~>* one-cr                                                        *)
-(* ------------------------------------------------------------------------- *)
-
-(*
-Local Lemma onecr_multistep_onecr_requires_acq' :
-  forall m1 m2 ths1 ths2 tid1 tid2 tc ad,
-    invariants m1 ths1 ->
-    invariants m2 ths2 ->
-    (* --- *)
-    tid1 <> tid2 ->
-    one_cr ad ths1[tid1] ->
-    m1 \ ths1 ~~[tc]~~>* m2 \ ths2 ->
-    one_cr ad ths2[tid2] ->
-    exists t, In (tid2, (e_acq ad t)) tc.
-Proof.
-  intros. ind_ustep.
-  - exfalso.
-    assert (Hucr : unique_holding m ths) by eauto with inva.
-    specialize (Hucr ad) as [Hfalse Htrue].
-    destruct (m[ad].X); spec.
-    + specialize Htrue as [tid [? ?]].
-      nat_eq_dec tid1 tid; nat_eq_dec tid2 tid;
-      eauto using nocr_onecr_contradiction.
-    + eauto using nocr_onecr_contradiction.
-  - assert (invariants m2 ths2) by eauto using invariants_preservation_ustep.
-    repeat spec.
-    assert (exists t, (e <> e_acq ad t /\ one_cr ad ths2[tid2]) \/
-                      (e =  e_acq ad t /\ tid = tid2))
-      as [t [[? ?] | [? ?]]]
-      by eauto using onecr_inheritance_cstep.
-    + destruct IHmultistep; trivial. eexists. right. eauto.
-    + subst. exists t. left. eauto.
-Qed.
-
-Local Corollary onecr_multistep_onecr_requires_acq :
-  forall m1 m2 ths1 ths2 tid1 tid2 tc ad,
-    invariants m1 ths1 ->
-    invariants m2 ths2 ->
-    (* --- *)
-    tid1 <> tid2 ->
-    one_cr ad ths1[tid1] ->
-    m1 \ ths1 ~~[tc]~~>* m2 \ ths2 ->
-    one_cr ad ths2[tid2] ->
-    exists t tc1 tc2, tc = tc2 ++ (tid2, e_acq ad t) :: tc1.
-Proof.
-  intros.
-  assert (exists t, In (tid2, (e_acq ad t)) tc)
-    as [t Hin] by eauto using onecr_multistep_onecr_requires_acq'.
-  apply in_split in Hin as [tc2 [tc1 Htc]].
-  exists t. exists tc1. exists tc2. assumption.
-Qed.
-
-Local Corollary multistep_acq_requires_unlocked :
-  forall m1 m2 ths1 ths2 tid1 tid2 tc1 tc2 ad t,
-    invariants m1 ths1 ->
-    invariants m2 ths2 ->
-    (* --- *)
-    tid1 <> tid2 ->
-    m1 \ ths1 ~~[tc2 ++ (tid2, e_acq ad t) :: tc1]~~>* m2 \ ths2 ->
-    exists mA thsA,
-      m1 \ ths1 ~~[tc1]~~>* mA \ thsA /\
-      mA[ad].X = false.
-Proof.
-  intros * ? ? ? H.
-  eapply destruct_ustep' in H. decompose record H.
-  repeat eexists; eauto.
-  invc_cstep. invc_cstep. invc_mstep. assumption.
-Qed.
-
-Local Lemma onecr_multistep_unlocked_requires_rel :
-  forall tc m1 m2 ths1 ths2 tid ad,
-    invariants m1 ths1 ->
-    invariants m2 ths2 ->
-    (* --- *)
-    one_cr ad ths1[tid] ->
-    m1 \ ths1 ~~[tc]~~>* m2 \ ths2 ->
-    m2[ad].X = false ->
-    In (tid, e_rel ad) tc.
-Proof.
-  intro. induction tc using rev_ind; intros.
-  - invc_ustep.
-    assert (unique_critical_regions m2 ths2) by eauto with inva.
-    assert (Htrue : m2[ad].X = true) by eauto using locked_from_onecr.
-    rewrite Htrue in *. auto.
-  - match goal with H : _ \ _ ~~[_ ++ ?e :: nil]~~>* _ \ _ |- _ => 
-      destruct e as [tid' e'];
-      eapply destruct_ustep' in H as [mA [mB [thsA [thsB [H1A [? ?]]]]]]
-    end.
-    invc H1A.
-    assert (invariants mB thsB) by eauto using invariants_preservation_cstep.
-    assert ((e' <> e_rel ad /\ one_cr ad thsB[tid]) \/
-            (e' =  e_rel ad /\ tid' = tid))
-      as [[? ?] | [? ?]]
-      by eauto using onecr_preservation_cstep;
-    subst; eauto using in_app_head, in_app_tail.
-Qed.
-
-Local Lemma onecr_multistep_onecr :
-  forall tc m1 m2 ths1 ths2 tid1 tid2 ad,
-    invariants m1 ths1 ->
-    invariants m2 ths2 ->
-    (* --- *)
-    tid1 <> tid2                   ->
-    one_cr ad ths1[tid1]           ->
-    m1 \ ths1 ~~[tc]~~>* m2 \ ths2 ->
-    one_cr ad ths2[tid2]           ->
-    exists tc1 tc2 t,
-      tc = tc2 ++ tc1           /\
-      In (tid1, e_rel ad)   tc1 /\
-      In (tid2, e_acq ad t) tc2.
-Proof.
-  intros.
-  assert (exists t tc1 tc2, tc = tc2 ++ (tid2, e_acq ad t) :: tc1)
-    as [t [tc1 [tc2 Hacq]]]
-    by eauto using onecr_multistep_onecr_requires_acq.
-  subst.
-  assert (exists mA thsA, m1 \ ths1 ~~[tc1]~~>* mA \ thsA /\ mA[ad].X = false)
-    as [mA [thsA [H1A Hunlocked]]]
-    by eauto using multistep_acq_requires_unlocked.
-  assert (invariants mA thsA) by eauto using invariants_preservation_ustep.
-  exists tc1. exists (tc2 ++ (tid2, e_acq ad t) :: nil). exists t.
-  repeat split; eauto using in_app_head, onecr_multistep_unlocked_requires_rel.
-  rewrite <- app_assoc. reflexivity.
-Qed.
-*)
-
-(* ------------------------------------------------------------------------- *)
-(* safety                                                                    *)
+(* safety -- final 1                                                         *)
 (* ------------------------------------------------------------------------- *)
 
 Local Ltac _preservation L :=
-  repeat (invc_cstep; invc_cstep; invc_mstep); sigma;
+  repeat (invc_cstep; invc_mstep); sigma;
   destruct_invariants; eauto using L.
 
-(*
-Theorem happens_before_from_gcrR :
-  forall m mA mB ths thsA thsB tid1 tid2 tc adx ad' t',
-    invariants m  ths  ->
-    invariants mA thsA ->
-    invariants mB thsB ->
-    (* --- *)
-    tid1 <> tid2                                    ->
-    gcr thsA[tid1] (R_tid tid1) = R_ad adx          ->
-    gcr thsB[tid2] (R_tid tid2) = R_ad adx          ->
-    mA \ thsA ~~~[tid1, e_read ad' t']~~> m  \ ths  ->
-    m  \ ths  ~~[tc]~~>*                  mB \ thsB ->
-    exists tc1 tc2, tc = tc2 ++ tc1 /\
-    exists adx t t',
-      (In (tid1, e_rel    adx)    tc1 /\ In (tid2, e_acq adx t) tc2) \/
-      (In (tid1, e_init adx t') tc1 /\ In (tid2, e_acq adx t) tc2).
-Proof.
-  intros * ? ? ? ? HgcrA HgcrB Hcstep Hustep.
-  assert (forall_memory mA value) by eauto with inva.
-  assert (forall_memory mA (valid_term mA)) by eauto with inva.
-  assert (no_inits t' /\ no_crs t') as [? ?]. {
-    invc_cstep; invc_cstep; invc_mstep;
-    split; eauto using noinits_from_value, nocrs_from_value.
-  }
-  assert (forall_threads thsA term_init_cr_exc) by eauto using des_inva_tice.
-  assert (forall_threads thsB term_init_cr_exc) by eauto using des_inva_tice.
-  eapply oneinit_or_onecr_from_gcr in HgcrA as [HoneinitA | HonecrA];
-  eapply oneinit_or_onecr_from_gcr in HgcrB as [HoneinitB | HonecrB];
-  eauto.
-  - assert (one_init adx ths[tid1]) by _preservation oneinit_preservation_read.
-    exfalso. eauto using oneinit_multistep_oneinit.
-  - assert (one_init adx ths[tid1]) by _preservation oneinit_preservation_read.
-    assert (exists tc1 tc2 t t',
-      tc = tc2 ++ tc1                /\
-      In (tid1, e_init adx t') tc1 /\
-      In (tid2, e_acq    adx t)     tc2)
-      as [tc1 [tc2 [t [t'' [? [? ?]]]]]]
-      by eauto using oneinit_multistep_onecr.
-    exists tc1, tc2. split; trivial.
-    repeat eexists. eauto.
-  - assert (one_cr adx ths[tid1]) by _preservation onecr_preservation_read.
-    exfalso. eauto using onecr_multistep_oneinit.
-  - assert (one_cr adx ths[tid1]) by _preservation onecr_preservation_read.
-    assert (exists tc1 tc2 t,
-      tc = tc2 ++ tc1            /\
-      In (tid1, e_rel adx)   tc1 /\
-      In (tid2, e_acq adx t) tc2)
-      as [tc1 [tc2 [t [? [? ?]]]]]
-      by eauto using onecr_multistep_onecr.
-    exists tc1, tc2. split; trivial.
-    eexists. eexists. exists <{unit}>. eauto.
-Qed.
-
-Theorem safety_write_read : forall m1 m2 ths1 ths2 tc tc' tid1 tid2 ad t1 t2,
-  tid1 <> tid2 ->
+Theorem happens_before_from_gcr : forall m1 m2 ths1 ths2 tid1 tid2 e1 e2 tc ad,
   invariants m1 ths1 ->
-  m1 \ ths1 ~~[tc]~~>* m2 \ ths2 ->
-  tc = (tid2, e_read ad t2) :: tc' +++ (tid1, e_write ad t1) ->
-  exists tc1 tc2, tc' = tc2 ++ tc1 /\
-  exists adx t t',
-    (In (tid1, e_rel    adx)    tc1 /\ In (tid2, e_acq adx t) tc2) \/
-    (In (tid1, e_init adx t') tc1 /\ In (tid2, e_acq adx t) tc2).
-Proof.
-  intros. subst. destruct_ustep3.
-  assert (invariants mA thsA) by eauto using invariants_preservation_cstep.
-  assert (invariants mB thsB) by eauto using invariants_preservation_ustep.
-  assert (invariants m2 ths2) by eauto using invariants_preservation_cstep.
-
-  assert (ad < #m1) by eauto using vtm_write_address_cstep.
-
-  assert (exists T, m1[ad].T = `w&T`)
-    as [T Hptyp1]
-    by eauto using cstep_ptyp_for_write.
-  assert (m1[ad].T = mA[ad].T /\ mA[ad].T = mB[ad].T /\ mB[ad].T = m2[ad].T)
-    as [HptypA [HptypB Hptyp2]]
-    by eauto using same_pointer_type.
-  rewrite Hptyp1 in HptypA. symmetry in HptypA.
-  rewrite HptypA in HptypB. symmetry in HptypB.
-  rewrite HptypB in Hptyp2. symmetry in Hptyp2.
-
-  assert (Hgcr1 : gcr ths1[tid1] (R_tid tid1) = m1[ad].R)
-    by eauto 7 using cstep_gcr_write with inva.
-  assert (HgcrB : gcr thsB[tid2] (R_tid tid2) = mB[ad].R)
-    by eauto using cstep_gcr_read with inva.
-
-  assert (HR : m1[ad].R = mB[ad].R) by eauto using same_regions.
-  rewrite <- HR in *.
-
-  destruct (m1[ad].R);
-  try solve [exfalso; eauto using gcr_tid_contradiction with gcr].
-
-  eauto using happens_before_from_gcrW.
-Qed.
-
-Corollary _rel_acq : forall m1 m2 ths1 ths2 tc1 tc2 e1 e2 tid1 tid2 adx t,
-  m1 \ ths1 ~~[(tid2, e2) :: (tc2 ++ tc1) +++ (tid1, e1)]~~>* m2 \ ths2 ->
-  In (tid1, e_rel adx) tc1 ->
-  In (tid2, e_acq adx t) tc2 ->
-  happens_before ((tid2, e2) :: (tc2 ++ tc1) +++ (tid1, e1)).
-Proof.
-  intros * Hustep Hin1 Hin2.
-  remember (tid1, e_rel adx) as evR.
-  remember (tid2, e_acq adx t) as evA.
-  apply in_split in Hin1 as [tcB [tcA Heq1]].
-  apply in_split in Hin2 as [tcD [tcC Heq2]].
-
-  unfold add.
-  rewrite <- app_assoc.
-  rewrite Heq1; clear Heq1.
-  rewrite <- app_assoc.
-  rewrite <- app_comm_cons.
-  rewrite app_assoc.
-  apply hb_trans.
-  - rewrite HeqevR. auto using happens_before.
-  - unfold add.
-    rewrite <- app_assoc.
-    rewrite Heq2; clear Heq2.
-    rewrite <- app_assoc.
-    rewrite <- app_comm_cons.
-    rewrite app_assoc.
-    apply hb_trans.
-    + rewrite HeqevA.
-      rewrite HeqevR.
-      auto using happens_before.
-    + rewrite HeqevA.
-      auto using happens_before.
-Qed.
-*)
-
-Notation "'<<' ev1 ',' tc ',' ev2 '>>'" := (ev2 :: tc +++ ev1).
-
-Local Corollary vtm_write_address_cstep : forall m1 m2 ths1 ths2 tid ad' t',
-  invariants m1 ths1 ->
+  invariants m2 ths2 ->
   (* --- *)
-  m1 \ ths1 ~~[tid, e_write ad' t']~~> m2 \ ths2 ->
-  ad' < #m1.
+  tid1 <> tid2                          ->
+  gcr ths1[tid1] (R_tid tid1) = R_ad ad ->
+  gcr ths2[tid2] (R_tid tid2) = R_ad ad ->
+  no_reacqs ths1[tid1]                  ->
+  no_reacqs ths2[tid2]                  ->
+  m1 \ ths1 ~~[tc]~~>* m2 \ ths2        ->
+  happens_before <<(tid1, e1), tc, (tid2, e2)>>.
 Proof.
-  intros * H ?.
-  eapply des_inva_vtm in H. eapply des_forallprogram_threads in H.
-  invc_cstep. invc_mstep. eauto using vtm_write_address.
-Qed.
-
-Theorem happens_before_from_gcrW :
-  forall m mA mB ths thsA thsB tid1 tid2 tc adx ad' t',
-    invariants m  ths  ->
-    invariants mA thsA ->
-    invariants mB thsB ->
-    (* --- *)
-    tid1 <> tid2                                    ->
-    gcr thsA[tid1] (R_tid tid1) = R_ad adx          ->
-    gcr thsB[tid2] (R_tid tid2) = R_ad adx          ->
-    mA \ thsA ~~[tid1, e_write ad' t']~~> m  \ ths  ->
-    m  \ ths  ~~[tc]~~>*                  mB \ thsB ->
-    exists tc1 tc2, tc = tc2 ++ tc1 /\
-    exists adx t t',
-      (In (tid1, e_rel    adx)    tc1 /\ In (tid2, e_acq adx t) tc2) \/
-      (In (tid1, e_init adx t') tc1 /\ In (tid2, e_acq adx t) tc2).
-Proof.
+  intros * ? ? ? Hgcr1 Hgcr2 ? ? Hustep.
+  assert (forall_threads ths1 term_init_cr_exc) by eauto with inva.
+  assert (forall_threads ths2 term_init_cr_exc) by eauto with inva.
+  assert (forall_threads ths1 (consistent_waits WR_none)) by eauto with inva.
+  assert (forall_threads ths2 (consistent_waits WR_none)) by eauto with inva.
+  eapply oneinit_or_onecr_from_gcr in Hgcr1 as [Honeinit1 | Honecr1];
+  eapply oneinit_or_onecr_from_gcr in Hgcr2 as [Honeinit2 | Honecr2];
+  eauto;
+  try solve
+    [ exfalso; eauto using oneinit_multistep_oneinit
+    | exfalso; eauto using onecr_multistep_oneinit
+  ].
+  - admit.
+  - admit.
   (*
-  intros * ? ? ? ? HgcrA HgcrB Hcstep Hustep.
-  assert (forall_threads thsA term_init_cr_exc) by eauto using des_inva_tice.
-  assert (forall_threads thsB term_init_cr_exc) by eauto using des_inva_tice.
-  eapply oneinit_or_onecr_from_gcr in HgcrA as [HoneinitA | HonecrA];
-  eapply oneinit_or_onecr_from_gcr in HgcrB as [HoneinitB | HonecrB];
-  eauto.
-  - assert (one_init adx ths[tid1]) by _preservation oneinit_preservation_write.
-    exfalso. eauto using oneinit_multistep_oneinit.
-  - assert (one_init adx ths[tid1]) by _preservation oneinit_preservation_write.
+  - (* aplicar hb_trans duas vezes *)
+    eapply hb_trans.
+
     assert (exists tc1 tc2 t t',
-      tc = tc2 ++ tc1                   /\
+      tc = tc2 ++ tc1                 /\
       In (tid1, e_init adx t') tc1    /\
       In (tid2, e_acq    adx t)     tc2)
       as [tc1 [tc2 [t [t'' [? [? ?]]]]]]
       by eauto using oneinit_multistep_onecr.
     exists tc1, tc2. split; trivial.
     repeat eexists. eauto.
-  - assert (one_cr adx ths[tid1]) by _preservation onecr_preservation_write.
-    exfalso. eauto using onecr_multistep_oneinit.
   - assert (one_cr adx ths[tid1]) by _preservation onecr_preservation_write.
     assert (exists tc1 tc2 t,
       tc = tc2 ++ tc1            /\
@@ -691,27 +408,71 @@ Proof.
   *)
 Abort.
 
-Lemma todo : forall tid ad t,
-  gcr t (R_tid tid) = R_reacq ad ->
+(* ------------------------------------------------------------------------- *)
+(* safety -- final 0                                                         *)
+(* ------------------------------------------------------------------------- *)
+
+Local Corollary vtm_write_address_cstep : forall m1 m2 ths1 ths2 tid ad' t',
+  invariants m1 ths1 ->
+  (* --- *)
+  m1 \ ths1 ~~[tid, e_write ad' t']~~> m2 \ ths2 ->
+  ad' < #m1.
+Proof.
+  intros * H ?.
+  eapply des_inva_vtm in H. eapply des_forallprogram_threads in H.
+  invc_cstep. invc_mstep. eauto using vtm_write_address.
+Qed.
+
+Lemma todo1 : forall R m t ad,
+  valid_term m t ->
+  (* -- *)
+  R <> R_reacq ad      ->
+  gcr t R = R_reacq ad ->
   waiting ad t.
 Proof.
-  intros. induction t; kappa; try discriminate; auto using waiting.
-  - repeat spec. eapply wg_plus1; eauto.
-Abort.
+  intros. gendep R.
+  induction t; intros; invc_vtm; kappa; try discriminate;
+  eauto using waiting;
+  match goal with
+  | H : _ _ (R_ad ?ad) = _          |- _ => spec; specialize (IHt (R_ad ad))
+  | H : R_reacq ?ad1 = R_reacq ?ad2 |- _ => invc H
+  end;
+  auto using waiting with gcr.
+Qed.
 
-(*
-Lemma todo : forall m1 m2 ths1 ths2 tid ad' t' ad,
+Lemma todo2 : forall m1 m2 ths1 ths2 tid ad ad' t',
+  waiting ad ths1[tid]                           ->
   m1 \ ths1 ~~[tid, e_write ad' t']~~> m2 \ ths2 ->
-  gcr ths1[tid] (R_tid tid) = R_reacq ad         ->
   False.
 Proof.
   intros. invc_cstep. invc_mstep.
   remember (ths1[tid]) as t1. clear Heqt1.
-  gendep t.
-  induction t1; intros; invc_tstep; kappa; try value_does_not_step.
-  - repeat spec.
+  ind_tstep; repeat invc_wg; auto; (value_does_not_step || value_does_not_wait).
 Qed.
-*)
+
+Lemma todo2' : forall m1 m2 ths1 ths2 tid ad' t',
+  forall_threads ths1 (valid_term m1) ->
+  (* --- *)
+  m1 \ ths1 ~~[tid, e_write ad' t']~~> m2 \ ths2 ->
+  no_reacqs ths1[tid].
+Proof.
+  intros * Hvtm **. invc_cstep. invc_mstep.
+  specialize (Hvtm tid).
+  remember (ths1[tid]) as t1. clear Heqt1.
+  ind_tstep; invc_vtm; try value_does_not_step;
+  repeat spec; intro; eauto using noreacq_from_value, no_reacq.
+Qed.
+
+Corollary todo3 : forall m1 m2 ths1 ths2 tid ad ad' t',
+  forall_threads ths1 (valid_term m1) ->
+  (* --- *)
+  gcr ths1[tid] (R_tid tid) = R_reacq ad         ->
+  m1 \ ths1 ~~[tid, e_write ad' t']~~> m2 \ ths2 ->
+  False.
+Proof.
+  assert (forall tid ad, R_tid tid <> R_reacq ad) by congruence.
+  eauto using todo1, todo2.
+Qed.
 
 Theorem safety_write_write : forall m1 m2 ths1 ths2 tc tc' tid1 tid2 ad t1 t2,
   invariants m1 ths1 ->
@@ -750,92 +511,6 @@ Proof.
   - exfalso. eauto using gcr_tid_contradiction with gcr.
   - exfalso. eauto using gcr_tid_contradiction with gcr.
   - admit.
-  - admit.
-
-  eauto using happens_before_from_gcrW.
+  - exfalso. eauto using todo3 with inva.
 Qed.
 
-Theorem safety_read_write : forall m1 m2 ths1 ths2 tc tc' tid1 tid2 ad t1 t2,
-  tid1 <> tid2 ->
-  invariants m1 ths1 ->
-  m1 \ ths1 ~~[tc]~~>* m2 \ ths2 ->
-  tc = (tid2, e_write ad t2) :: tc' +++ (tid1, e_read ad t1) ->
-  exists tc1 tc2, tc' = tc2 ++ tc1 /\
-  exists adx t t',
-    (In (tid1, e_rel  adx)    tc1 /\ In (tid2, e_acq adx t) tc2) \/
-    (In (tid1, e_init adx t') tc1 /\ In (tid2, e_acq adx t) tc2).
-Proof.
-  intros. subst. destruct_ustep3.
-  assert (invariants mA thsA) by eauto using invariants_preservation_cstep.
-  assert (invariants mB thsB) by eauto using invariants_preservation_ustep.
-  assert (invariants m2 ths2) by eauto using invariants_preservation_cstep.
-
-  assert (ad < #m1) by (repeat (invc_cstep; invc_cstep; invc_mstep); trivial).
-
-  assert (exists T, mB[ad].T = `w&T`)
-    as [T HptypB]
-    by eauto using cstep_ptyp_for_write.
-  assert (m1[ad].T = mA[ad].T /\ mA[ad].T = mB[ad].T /\ mB[ad].T = m2[ad].T)
-    as [Hptyp1 [HptypA _]]
-    by eauto using same_pointer_type.
-  rewrite HptypB in HptypA.
-  rewrite HptypA in Hptyp1.
-
-  assert (Hgcr1 : gcr ths1[tid1] (R_tid tid1) = m1[ad].R)
-    by eauto   using cstep_gcr_read with inva.
-  assert (HgcrB : gcr thsB[tid2] (R_tid tid2) = mB[ad].R)
-    by eauto 7 using cstep_gcr_write with inva.
-
-  assert (HR : m1[ad].R = mB[ad].R) by eauto using same_regions.
-  rewrite <- HR in *.
-
-  destruct (m1[ad].R);
-  try solve [exfalso; eauto using gcr_tid_contradiction with gcr].
-
-  eauto using happens_before_from_gcrR.
-Qed.
-
-(* ------------------------------------------------------------------------- *)
-(*                                                                           *)
-(* ------------------------------------------------------------------------- *)
-
-Theorem write_happens_before_read :
-  forall m1 m2 ths1 ths2 tc tc' tid1 tid2 ad t1 t2,
-    invariants m1 ths1 ->
-    m1 \ ths1 ~~[tc]~~>* m2 \ ths2 ->
-    tc = (tid2, e_read ad t2) :: tc' +++ (tid1, e_write ad t1) ->
-    happens_before tc.
-Proof.
-  intros. subst. nat_eq_dec tid1 tid2; auto using happens_before.
-
-
-  destruct_ustep3.
-  assert (invariants mA thsA) by eauto using invariants_preservation_cstep.
-  assert (invariants mB thsB) by eauto using invariants_preservation_ustep.
-  assert (invariants m2 ths2) by eauto using invariants_preservation_cstep.
-
-  assert (ad < #m1) by eauto using vtm_write_address_cstep.
-
-  assert (exists T, m1[ad].T = `w&T`)
-    as [T Hptyp1]
-    by eauto using cstep_ptyp_for_write.
-  assert (m1[ad].T = mA[ad].T /\ mA[ad].T = mB[ad].T /\ mB[ad].T = m2[ad].T)
-    as [HptypA [HptypB Hptyp2]]
-    by eauto using same_pointer_type.
-  rewrite Hptyp1 in HptypA. symmetry in HptypA.
-  rewrite HptypA in HptypB. symmetry in HptypB.
-  rewrite HptypB in Hptyp2. symmetry in Hptyp2.
-
-  assert (Hgcr1 : gcr ths1[tid1] (R_tid tid1) = m1[ad].R)
-    by eauto 7 using cstep_gcr_write with inva.
-  assert (HgcrB : gcr thsB[tid2] (R_tid tid2) = mB[ad].R)
-    by eauto using cstep_gcr_read with inva.
-
-  assert (HR : m1[ad].R = mB[ad].R) by eauto using same_regions.
-  rewrite <- HR in *.
-
-  destruct (m1[ad].R);
-  try solve [exfalso; eauto using gcr_tid_contradiction with gcr].
-
-  eauto using happens_before_from_gcrW.
-Qed.
